<article>

# Gamma function

## Euler product

Not only did Euler come up with the integral form, he also produced a product formula, which we will investigate.

The formula is:
$$\Gamma(z)=\lim_{n\rightarrow\infty}\frac{n!n^z}{\prod\limits_{m=0}^n(z+m)}$$
We note that the denominator displays explicitly the pole singularities of the function at zero and the negative integers. So long as the limit converges (and it does), we have a definition all z, except for these singular points.

We have to show that this is equivalent (for $\mathrm{Re(z)}>0$) to the integral. A halfway post stop is to note that:
$$\frac{n!n^z}{\prod\limits_{m=0}^n(z+m)}=\int_0^n t^{z-1}\left(1-\frac t n\right)^ndt$$
This is shown by integrating by parts $n$ times, increasing each time the power by 1 on the $t$ factor and decreasing by 1 on the $(1-t/n)$ part. The integrated surface terms are zero until one reaches:
$$\int_0^n t^{z-1}\left(1-\frac t n\right)^ndt=\frac{n!}{\prod\limits_{m=0}^{n-1}(z+m)}\int_0^nt^{z+n-1}dt$$
The final simple integral completes the product formula. The numerator comes from the differentiating, and the denominator from the integrating.

If we could just swap the order of the integral and limit, we could simply replace $(1-t/n)^n$ by $\exp(-t)$ and we would be finished. There are theorems in integration theory, but improper integrals are a pain in this respect. Finite bits can slink off to infinity and apparently disappear, while still adding a extra finite contribution to the integral. We have to show that that doesnâ€™t happen.

First we note $\exp(t)\ge 1+t$ for all real $t$. This can be demonstrated by showing that the minimum of $\exp(t)-t$ is 1, which is the value at $t=0$. We can swap the sign of $t$ to give $\exp(-t)\ge 1-t$ Hence:
$$\exp(t)\left(1-\frac t n\right)^n\le \exp(t)(\exp(t/n))^n=1$$
In the other direction:
$$\exp(t)\left(1-\frac t n\right)^n\ge \left(1+\frac t n\right)^n\left(1-\frac t n\right)^n=\left(1-\frac {t^2} {n^2}\right)^n$$

We also have $(1-t)^n\ge 1-nt$, at least for $t \le 2$, by a similar argument as for the exponential. Hence:
$$1-\frac{t^2}n\le\exp(t)\left(1-\frac t n\right)^n\le 1$$
for $0\le t\le n$

Some rearrangement:
$$0\le1-\exp(t)\left(1-\frac t n\right)^n\le\frac{t^2}n$$

Multiplying by $\exp(-t)$:
$$0\le\exp(-t)-\left(1-\frac t n\right)^n\le\frac{t^2}n\exp(-t)$$

This allows us to show that, for $\mathrm{Re}(z)\gt0$:
$$\lim_{n\rightarrow\infty} \int\limits_0^n\left|\exp(-t)-\left(1-\frac t n\right)^n\right|
\left|t^{z-1}\right|
dt\le \\ \lim_{n\rightarrow\infty}\int\limits_0^\infty\frac{t^{2+\mathrm{Re}(z)-1}}n\exp(-t)dt=\frac{\Gamma(2+\mathrm{Re}(z))}n\rightarrow0$$
This gives us, after some standard arguments:
$$
\begin{aligned}
\Gamma(z)&=\lim_{n\rightarrow\infty}\int_0^n t^{z-1}\left(1-\frac t n\right)^ndt \\
&=\lim_{n\rightarrow\infty}\frac{n!n^z}{\prod\limits_{m=0}^n(z+m)}
\end{aligned}
$$
</article>