<article>

# Gamma function

## Logarithmic interlude

We note that:
$$\ln(z)=\int\limits_0^\infty\frac{\exp(-t)-\exp(-tz)}tdt$$

First, when $z=1$ $\ln(z)$ and the integral are both zero. The integral converges at both limits. In particular, the integrand tends continuiously to $z-1$ as $t\rightarrow 0$.

Second, the first derivatives of the two sides are equal to $1/z$. For the logarithm, this is almost by definition. For the integral, we can swap the order of differentiaion and integration to give:
$$\int\limits_0^\infty\frac{d}{dz}\left[\frac{\exp(-t)-\exp(-tz)}t\right]dt= \\ \int\limits_0^\infty\exp(-tz)dt=\frac 1 z$$

The difference between the two objects therefore does not change from its value 0 at $z=1$. In fact, we could integrate the integral representation of $1/z$ from 1 to get our representation:
$$\ln(z)=\int\limits_1^z\frac 1zdz=\int\limits_1^z\int\limits_0^\infty\exp(-tz)dtdz$$
Swapping the integral order:
$$\ln(z)= \\
\int\limits_0^\infty\int\limits_1^z\exp(-tz)dzdt= \\
\int\limits_0^\infty\left[\frac{\exp(-tz)}{-t}\right]_1^zdt= \\
\int\limits_0^\infty\left[\frac{\exp(-t)-\exp(-tz)}{t}\right]dt$$
which is easily seen to be our headline result.
</article>