<article>

# Gamma function

## An extraction

We can use the logarithmic interlude to extract some nastiness from $\psi$:
$$\psi(z)-\ln(z)= \\
\int\limits_0^\infty\left[\frac{\exp(-t)}t-\frac{\exp(-zt)}{1-\exp(-t)}\right]dt- \\
\int\limits_0^\infty\frac{\exp(-t)-\exp(-tz)}tdt= \\
\int\limits_0^\infty\left[\frac{1}t-\frac{1}{1-\exp(-t)}\right]\exp(-zt)dt$$
The bracket varies from $-1/2$ at $t=0$, to $-1$ as $t\rightarrow\infty$. We will see that when we want a formula for $\ln\Gamma(z)$ that it will be useful to remove the constant at $t=0$. The necessary extraction is:
$$\frac1{2z}=\int\limits_0^\infty\frac1 2\exp(-zt)dt$$
Adding this in we get:
$$\psi(z)-\ln(z)+\frac1{2z}= \\
\int\limits_0^\infty\left[\frac1 2+\frac{1}t-\frac{1}{1-\exp(-t)}\right]\exp(-zt)dt$$

An alternative is:
$$\frac1 2+\frac{1}t-\frac{1}{1-\exp(-t)}=\\
\frac1 2+\frac{1}t-\frac{\exp(t)}{\exp(t)-1}=\\
\frac1 2+\frac{1}t-\frac{\exp(t)-1+1}{\exp(t)-1}=\\
\frac{1}t-\frac1 2-\frac{1}{\exp(t)-1}$$
This is the form used in Binet’s “first expression” for $\ln\Gamma(z)$.
</article>