<article>

# Gamma function
## Binet 1 constant

We have defined the integral:
$$I(z)=\int\limits_0^\infty\left[\frac1 2-\frac1t+\frac{1}{\exp(t)-1}\right]\frac{\exp(-zt)}{t}dt$$
and we want to evaluate $I(1)$. We know that:
$$\ln\Gamma(z)=(z-\tfrac12)\ln(z)-z+1+I(z)-I(1)$$
We also happen to know that $\Gamma(1/2)=\sqrt\pi$. This gives:
$$\tfrac12\ln(\pi)=\tfrac12+I(\tfrac12)-I(1)$$

Let’s look at $I(1)$:
$$I(1)=\int\limits_0^\infty\left[\frac1 2-\frac1t+\frac{1}{\exp(t)-1}\right]\frac{\exp(-t)}{t}dt$$
We can make it look more like $I(1/2)$ by a change of variable $t\rightarrow t/2$:
$$I(1)=\int\limits_0^\infty\left[\frac1 2-\frac2t+\frac{1}{\exp(t/2)-1}\right]\frac{\exp(-t/2)}{t}dt$$
We can make the third term in bracket more acceptable for comparison by:
$$\frac{1}{\exp(t/2)-1}=\frac{1}{\exp(t/2)-1}\frac{\exp(t/2)+1}{\exp(t/2)+1}=\frac{\exp(t/2)+1}{\exp(t)-1}$$

We can extract a term of $I(1/2)$:
$$I(1)=I(\tfrac12)+\int\limits_0^\infty\left[-\frac2t+\frac{\exp(t/2)}{\exp(t)-1}\right]\frac{\exp(-t/2)}{t}dt= \\
I(\tfrac12)+\int\limits_0^\infty\left[-\frac{\exp(-t/2)}t+\frac1{\exp(t)-1}\right]\frac{dt}{t}$$

So:
$$I(\tfrac12)=I(1)-\int\limits_0^\infty\left[-\frac{\exp(-t/2)}t+\frac1{\exp(t)-1}\right]\frac{dt}{t}= \\
\int\limits_0^\infty\left[\tfrac12\exp(-t)-\frac{\exp(-t)}t+ \frac{\exp(-t)}{\exp(t)-1}+ \right.\\ \left.
\frac{\exp(-t/2)}t-\frac1{\exp(t)-1}\right]\frac{dt}{t}
$$
We can combine:
$$\frac{\exp(-t)}{\exp(t)-1}-\frac1{\exp(t)-1}=\frac{\exp(-t)-1}{\exp(t)-1}=-\exp(-t)$$
Thus:
$$I(\tfrac12)=\int\limits_0^\infty\left[\frac{\exp(-t/2)-\exp(-t)}t-\tfrac12\exp(-t)\right]\frac{dt}{t}$$
We integrate by parts the more singular first term of the square bracket:
$$I(\tfrac12)=-\left[\frac{\exp(-t/2)-\exp(-t)}t\right]_0^\infty+ \\ \tfrac12\int\limits_0^\infty\left[\exp(-t)-\exp(-t/2)\right]\frac{dt}{t}$$
The integrated part is 1/2, and the integral is our logarithmic interlude evaluated at 1/2:
$$I(\tfrac12)=\tfrac12+\tfrac12\ln(\tfrac12)$$

Remembering:
$$\tfrac12\ln(\pi)=\tfrac12+I(\tfrac12)-I(1)$$
we get:
$$I(1)=\tfrac12+I(\tfrac12)-\tfrac12\ln(\pi)=1+\tfrac12\ln(\tfrac12)-\tfrac12\ln(\pi)$$
But remembering that $\ln(1/2)=-\ln(2)$, and $\ln(2)+\ln(\pi)=\ln(2\pi)$:
$$I(1)=1-\tfrac12\ln(2\pi)$$
So _finally_:
$$\ln\Gamma(z)=(z-\tfrac12)\ln(z)-z+\tfrac12\ln(2\pi)+I(z)$$
with
$$I(z)=\int\limits_0^\infty\left[\frac1 2-\frac1t+\frac{1}{\exp(t)-1}\right]\frac{\exp(-zt)}{t}dt$$
We’ll not get into _Binet 2_ for now, since the derivation involves too much contour integration, so far as I can see, with little apparent payoff.
</article>