<article>

# Difference operators

## Backward


The relation between $D=d/dx$ and $\nabla=1-T^{-1}$, where $[Tp](x)=p(x+1)$, is given by Taylor series that can be compacted into:

$$\exp(-D)=T^{-1}=1-\nabla$$

We also have $[\exp(xD)p](n)=p(n+x)=[(1-\nabla)^{-x}p](n)$. We can formally binomial expand:

$$p(n+x)=[(1-\nabla)^{-x}p](n)=\sum\limits_{k=0}^\infty \binom{-x}k (-1)^k [\nabla^kp](n)$$

From the operator expansion:

$$S=\sum[Sq_k](0)Q^k$$

applied to $T^x$:

$$T^x=\sum[T^xq_k](0)\nabla^k=\sum q_k(x)\nabla^k$$

we read off the basic polynomials for $\nabla$:

$$q_k(x)=\binom{-x}k (-1)^k$$

This gives $q_0(x)=1$.

A more specific formula is:

$$q_k(x)=\frac1{k!}\prod\limits_{n=0}^{k-1}(x+n)$$

This makes it fairly easy to confirm $\nabla q_k=q_{k-1}.$

 </article>