<article>

# Delta force

## Introduction

To recap delta operators are shift invariant, reduce constants to zero and linear polynomials to a constant. Further $Q$ reduces the degree of polynomials by 1.

We define a basic sequence of polynomials for $Q$:

1. $q_0(x)=1$

2. $q_n(0)=0,n>0$

3. $Qq_n=q_{n-1},n>0$

These conditions show that $q_n$ has degree $n$.

We can construct the sequence, starting from $q_0(x)=1$.

With $Q=\sum b_kD^k$, with $b_0=0$, $b_1\ne0$, and $q_n(x)=\sum\beta_{nl}x^l$:

$$Qq_n(x)=\sum b_k\beta_{nl}D^kx^l=\sum b_k\beta_{nl}\frac{l!}{(l-k)!}x^{l-k}$$

We need to collect the terms and equate to $q_{n-1}$:

$$\beta_{(n-1)l}=\sum\limits_{k=1}^{n-l}\frac{(l+k)!}{l!}b_k\beta_{n(l+k)}$$

We get immediately $\beta_{(n-1)(n-1)}=nb_1\beta_{nn}$.

Inserting in the equation for $\beta_{(n-1)(n-2)}$ determines $\beta_{n(n-1)}$ and so on, giving a polynomial $q_n$ uniquely determined from $q_{n-1}$.

The basic sequence is of convolution type:

1. $q_0(x)=1$

2. If $f(x)=q_{n}(x+y)-\sum q_k(x)q_{n-k}(y)$, then $[Qf](x)=q_{n-1}(x+y)-\sum q_k(x)q_{n-1-k}(x)$, shifting the $k$ index by 1.
$[Qq_n(x+y)=T^yQq_n(x)=T^yq_{n-1}(x)=q_{n-1}(x+y)$ since $Q$ is shift invariant.]


If the sequence satisfies the convolution identity for $q_{n-1}$, we have $Qf=0$. This means that $f$ is a constant, since $Q$ is a delta operator. But $f(0)=q_n(y)-q_n(y)=0$, since $q_n$ is a basic sequence. Hence the constant is zero, and $q_n$ also satisfies the convolution identity.

To complete the inductive proof, we just note that $q_0(x+y)=q_0(x)q_0(y)=1$ trivially satisfies the convolution identity.

A convolution sequence can be used to define a delta operator via $Qq_n=q_{n-1}$. The convolution property provides shift-invariance.

</article>