<article>

# Delta force

## Basic training

We define a derivative of shift-invariant operators, first given by Pincherle:

$$S'=[S,\mathbf x]$$

where $\mathbf x$ is the multiplication by $x$ operator, $\mathbf x p(x)=xp(x)$. Clearly, $(S_1+S_2)'=S_1'+S_2'$.

We have $D'=1$. From commutator theory,

$$[S_1S_2,S_3]=S_1S_2S_3-S_3S_1S_2=S_1[S_2,S_3]+S_1S_3S_2-S_3S_1S_2=S_1[S_2,S_3]+[S_1,S_3]S_2$$

Thus $(S_1S_2)'=S_1S_2'+S_1'S_2$, giving a _derivation_ (Leibnitz rule). Applying to $(D^k)'=D^{k-1}+D(D^{k-1})'$, an inductive proof shows $(D^k)'=kD^{k-1}$. A shift-invariant operator is expressible in terms of $D$, its derivative is also, and is shift-invariant too.

The derivative of a delta operator, $Q'$ has non-zero constant part in terms of $D$. This implies that it is invertible.

Further

$$Q=\sum\limits_{k=1}^\infty b_kD^k=D\sum\limits_{k=0}^\infty b_{k+1}D^k=DU$$

where $U$ is an invertible operator.

We look at $p_n(x)=Q'U^{-n-1}x^n/n!$. Remembering shift-invariant operators commute,

$$Qp_n(x)=DUQ'U^{-n-1}\frac{x^n}{n!}=Q'U^{-n}D\frac{x^n}{n!}=Q'U^{-n}\frac{x^{n-1}}{(n-1)!}=p_{n-1}(x)$$

To show that $p_n$ is the basic sequence for $Q$, we need to find its evaluations at 0.

For this we look at alternative expresssions. We start from $Q'=(DU)'=D'U+DU'=U+DU'$ since $D'=1$.

$$p_n(x)=Q'U^{-n-1}\frac{x^n}{n!}=U^{-n}\frac{x^n}{n!}+U'U^{-n-1}\frac{x^{n-1}}{(n-1)!}$$

When $n=0$,the second term is zero, so $p_0(x)=U^0x^0/0!=1$.

Also we have $(U^n)'=nU'U^{n-1}$. In our case we are interested in $U'U^{-n-1}=-(U^{-n})'/n$, giving

$$p_n(x)=U^{-n}\frac{x^n}{n!}-(U^{-n})'\frac{x^{n-1}}{n!}$$

Remembering the Pincherle derivative is the commutator with $\mathbf x$:

$$p_n(x)=U^{-n}\frac{x^n}{n!}-[U^{-n},\mathbf x]\frac{x^{n-1}}{n!}=\mathbf xU^{-n}\frac{x^{n-1}}{n!}$$

This shows that $p_n(0)=0$, at least for $n>0$. Completing the proof that $p_n=q_n$, the basic sequence of $Q$.

So making the replacement:

1. $q_n(x)=Q'U^{-n-1}\dfrac{x^n}{n!}$

2. $q_n(x)=U^{-n}\dfrac{x^n}{n!}-(U^{-n})'\frac{x^{n-1}}{n!}$

3. $q_n(x)=\mathbf xU^{-n}\dfrac{x^{n-1}}{n!}$

Remembering that $Q'$ is invertible:

$$\frac{x^{n-1}}{(n-1)!}=Q'^{-1}U^nq_{n-1}$$

giving

4. $q_n(x)=\mathbf x Q'^{-1}\dfrac{q_{n-1}}{n}$

From the polynomial expansion formula:

$$\frac{q_n(x)}x=\sum\limits_{k=0}^n\left[Q^k\frac{q_n(x)}x\right](0)q_k(x)$$

$$\frac{q_n(x)}x=\sum\limits_{k=0}^n\left[Q^kQ'^{-1}\dfrac{q_{n-1}}{n}\right](0)q_k(x)$$

$$\frac{q_n(x)}x=\sum\limits_{k=0}^n\left[Q'^{-1}\dfrac{q_{n-1-k}}{n}\right](0)q_k(x)$$

$$\frac{q_n(x)}x=\sum\limits_{k=0}^n\left[(n-k)\dfrac{q_{n-k}}{nx}\right](0)q_k(x)$$

The value of $q_n/x$ at zero is $q_n'(0)$, which is also given by the convolution-type coefficient sequence $\alpha_n=q_n'(0)$.

5. $q_n(x)=\dfrac xn\sum\limits_{k=1}^{n-1}k\alpha_k q_{n-k}(x)$

</article>